\documentclass[14pt]{extreport}
\usepackage[letterpaper, margin=1in]{geometry}
\usepackage{setspace}
\usepackage[dvipsnames]{xcolor}
\usepackage{ragged2e}
\usepackage{amsmath}
\usepackage{cancel}
\usepackage{multicol}
\usepackage{multirow}
\usepackage{fancyhdr}
\pagestyle{fancy}
\usepackage{lastpage} 
\usepackage{xcolor,colortbl}
\usepackage{amssymb}
\usepackage{graphicx}

\lhead{April 3, 2021}
\chead{}
\rhead{jnrozano@up.edu.ph}

\lfoot{Jhon Christian N. Rozano}
\cfoot{}
\rfoot{Page \thepage\ of \pageref{LastPage}}

\renewcommand{\headrulewidth}{1pt}

\renewcommand{\footrulewidth}{1pt}

\newcommand*\Eval[3]{\left.#1\right\rvert_{#2}^{#3}}

\definecolor{LightCyan}{rgb}{0.88,1,1}

\begin{document}
	\setlength{\columnsep}{20pt}
	\renewcommand{\arraystretch}{1.5}
	\singlespacing
	
	\noindent
	\begin{center}
		{\large  \textbf{Math Problem of the Day}} \\ 
	\end{center}
	
		\noindent
		Calculate the limit below in terms of $a$, and $b$, where $a$, and $b$ are constants with $b \geq 0$.
		\[ \lim_{n \to \infty} {\left( \frac{a + \sqrt[n]{b} - 1}{a}  \right)}^n  \]
	\bigskip
	\noindent
	\textbf{Solution:} \\
		Set the expression to $y$ and take the natural logarithm of both sides, we have
		\[ y = \lim_{n \to \infty} {\left( \frac{a + \sqrt[n]{b} - 1}{a}  \right)}^n  \Rightarrow
 		\ln y = \lim_{n \to \infty} n \ln \left( \frac{a + \sqrt[n]{b} - 1}{a}  \right)
 		=  \lim_{n \to \infty} \frac{ \ln \left( \frac{a + \sqrt[n]{b} - 1}{a}  \right)}{\frac{1}{n}} \]
		Let $ p = \frac{1}{n}  $, then the expression becomes
		\[  \lim_{p \to 0} \frac{ \ln \left( \frac{a + b^p - 1}{a}  \right)}{p} = \ln y \]
		Note that the limit above will be indeterminate in the form $\frac{0}{0}$ as $ p \to 0  $. Thus, using the L'HÃ´pital's rule,
		\[  \lim_{p \to 0} \frac{ \ln \left( \frac{a + b^p - 1}{a}  \right)}{p} =  \lim_{ p \to 0 } \left[ \frac{  \frac{\mathrm{d}}{\mathrm{d}p} \left( \frac{a + b^p - 1}{a} \right)  }{1 \cdot \frac{a + b^p - 1}{a}} \right] = \lim_{ p \to 0} \left( \frac{a}{a+b^p-1} \cdot \frac{b^p \ln b}{a} \right) \]
		\[ \lim_{ p \to 0} \left( \frac{a}{a+b^p-1} \cdot \frac{b^p \ln b}{a} \right) = \frac{\ln b}{a} = \ln y \]
		Hence,
		\[ y = e^{\ln b^{\frac{1}{a}}} = b^{\frac{1}{a}} =\textcolor{red}{\sqrt[a]{b}}  \]

\end{document}
